Update persistently lecture

go/memoize/memoize.go
@@ -1,5 +1,8 @@
 package memoize
 
+import "github.com/goose-lang/primitive"
+
+// Memoize wraps a (slow) function and caches its results
 type Memoize struct {
 	f       func(uint64) uint64
 	results map[uint64]uint64
@@ -20,6 +23,36 @@ func (m Memoize) Call(x uint64) uint64 {
 	y := m.f(x)
 	m.results[x] = y
 	return y
+}
+
+func UseMemoize1() {
+	m := NewMemoize(func(x uint64) uint64 {
+		return x * x
+	})
+	y1 := m.Call(3)
+	primitive.Assert(y1 == 9)
+	y2 := m.Call(3)
+	primitive.Assert(y2 == 9)
+	y3 := m.Call(5)
+	primitive.Assert(y3 == 25)
+}
+
+func UseMemoize2(s []uint64) {
+	sumUpto := func(n uint64) uint64 {
+		if n > uint64(len(s)) {
+			return 0
+		}
+		var sum uint64
+		for i := uint64(0); i < n; i++ {
+			sum += s[i]
+		}
+		return sum
+	}
+
+	m := NewMemoize(sumUpto)
+	y1 := m.Call(3)
+	y2 := m.Call(3)
+	primitive.Assert(y1 == y2)
 }
 
 // MockMemoize has the same API as Memoize but with an implementation that
